Add substitution to hypotheses.

logic/logic_aux_lemmas.v
@@ -12,7 +12,7 @@ Lemma heq_cases_ceq Σ D Γ Ψ h1 h2 op A B c1 c2 :
   form Γ Ψ (Heq Σ D h1 h2) -> get_op_type Σ op = Some (A, B) ->
   get_case h1 op = Some c1 ->
   get_case h2 op = Some c2 ->
-  form (CtxU (CtxU Γ (TyFun B D)) A) Ψ (Ceq D c1 c2).
+  form (CtxU (CtxU Γ (TyFun B D)) A) (hyp_shift Ψ 2 0) (Ceq D c1 c2).
 Proof.
 intros eqs gets finds1 finds2.
 induction Σ. simpl in gets. discriminate.
@@ -47,7 +47,8 @@ intros wf sty. induction Σ' as [ | Σ' IH o A' B'].
   destruct case2 as [c2 find2].
   clear A1 B1 get1 A2 B2 get2.
   eapply HeqSigU; eauto.
-  assert (form (CtxU (CtxU Γ (TyFun B'0 D)) A'0) Ψ (Ceq D c1 c2)).
+  assert 
+    (form (CtxU (CtxU Γ (TyFun B'0 D)) A'0) (hyp_shift Ψ 2 0) (Ceq D c1 c2)).
   - eapply heq_cases_ceq. 2: eauto. all: eauto.
     eapply WfForm; eauto. eapply WfHeq. 2: exact H8. all: eauto.
   - eapply ctx_subtype_form; eauto.
@@ -56,30 +57,35 @@ intros wf sty. induction Σ' as [ | Σ' IH o A' B'].
       all: inv H10; (apply ctx_subtype_refl || apply csubtype_refl); auto.
 Qed.
 
-
-Fixpoint veq_subtype A A' Γ Ψ v1 v2 
-  (orig: form Γ Ψ (Veq A v1 v2)) {struct orig} :
+(* This formulation is needed so that the termination
+   checker doesnt run forever. *)
+Fixpoint veq_subtype Γ Ψ judg (orig: form Γ Ψ judg) A A' v1 v2 {struct orig} :
+  judg = Veq A v1 v2 ->
   wf_vtype A' -> vsubtype A A' -> 
   form Γ Ψ (Veq A' v1 v2)
-with ceq_subtype C C' Γ Ψ c1 c2 
-  (orig: form Γ Ψ (Ceq C c1 c2)) {struct orig} :
+with ceq_subtype Γ Ψ judg (orig: form Γ Ψ judg) C C' c1 c2 {struct orig} :
+  judg = Ceq C c1 c2 ->
   wf_ctype C' -> csubtype C C' -> 
   form Γ Ψ (Ceq C' c1 c2).
 Proof.
 { 
-intros wfa' stya. inv orig. inv H.
-assert (wf_ctx Γ) as wfctx by (inv H5; assumption).
+intros same wfa' stya.
+assert (wf_ctx Γ) as wfctx.
+{ clear veq_subtype ceq_subtype. inv orig. inv H. inv H5. auto. } 
 assert (has_vtype Γ v1 A') as ty1.
-{ apply TypeV; auto. eapply TypeVSubtype; eauto. }
+{ clear veq_subtype ceq_subtype. inv orig. inv H.
+  apply TypeV; auto. eapply TypeVSubtype; eauto. }
 assert (has_vtype Γ v2 A') as ty2.
-{ apply TypeV; auto. eapply TypeVSubtype; eauto. }
+{ clear veq_subtype ceq_subtype. inv orig. inv H.
+  apply TypeV; auto. eapply TypeVSubtype; eauto. }
 apply WfForm; auto. apply WfVeq; auto.
-inv H1.
-+ specialize (veq_subtype _ A' _ _ _ _ H4) as IH.
+{ clear veq_subtype ceq_subtype. inv orig. auto. }
+destruct orig. destruct H1; inv same.
++ specialize (veq_subtype _ _ _ H1) as IH.
   clear veq_subtype ceq_subtype.
   apply VeqSym. eauto.
-+ specialize (veq_subtype _ A' _ _ _ _ H6) as IH1.
-  specialize (veq_subtype _ A' _ _ _ _ H9) as IH2.
++ specialize (veq_subtype _ _ _ H1) as IH1.
+  specialize (veq_subtype _ _ _ H2) as IH2.
   clear veq_subtype ceq_subtype.
   eapply VeqTrans; eauto.
 + clear veq_subtype ceq_subtype.
@@ -89,39 +95,40 @@ inv H1.
 + clear veq_subtype ceq_subtype. 
   inv stya. apply VeqInt; eauto.
 + inv stya.
-  specialize (veq_subtype _ A'0 _ _ _ _ H6) as IH1.
-  specialize (veq_subtype _ B' _ _ _ _ H9) as IH2.
+  specialize (veq_subtype _ _ _ H1) as IH1.
+  specialize (veq_subtype _ _ _ H2) as IH2.
   clear veq_subtype ceq_subtype.
   inv wfa'. eapply VeqPair; eauto.
 + inv stya. 
-  specialize (veq_subtype _ A'0 _ _ _ _ H4) as IH2.
+  specialize (veq_subtype _ _ _ H1) as IH.
   clear veq_subtype ceq_subtype.
   inv wfa'. eapply VeqInl; eauto.
 + inv stya.
-  specialize (veq_subtype _ B' _ _ _ _ H4) as IH2.
+  specialize (veq_subtype _ _ _ H1) as IH.
   clear veq_subtype ceq_subtype.
   inv wfa'. eapply VeqInr; eauto.
 + clear veq_subtype ceq_subtype. 
   inv stya. eapply VeqListNil.
 + inv stya. 
-  specialize (veq_subtype _ A'0 _ _ _ _ H6) as IH1.
-  specialize (veq_subtype _ (TyList A'0) _ _ _ _ H9) as IH2.
+  specialize (veq_subtype _ _ _ H1) as IH1.
+  specialize (veq_subtype _ _ _ H2) as IH2.
   clear veq_subtype ceq_subtype.
-  inv wfa'. eapply VeqListCons; eauto. apply IH2.
-  apply WfTyList. auto.
+  inv wfa'. eapply VeqListCons; eauto.
+  eapply IH2. eauto.
+  apply WfTyList. auto. 
   apply SubtypeTyList. auto.
 + inv stya.
-  specialize (ceq_subtype _ C' _ _ _ _ H4) as IH.
+  specialize (ceq_subtype _ _ _ H1) as IH.
   clear veq_subtype ceq_subtype.
   inv wfa'. apply VeqFun.
   eapply ctx_subtype_form. eauto.
   - apply WfCtxU; auto.
   - apply SubtypeCtxU; auto. apply ctx_subtype_refl. auto.
 + inv stya.
-  specialize (ceq_subtype _ D'0 _ _ _ _ H8) as IH.
+  specialize (ceq_subtype _ _ _ H1) as IH.
   clear veq_subtype ceq_subtype.
-  inv wfa'. inv H2. inv H3. eapply VeqHandler.
-  eapply ctx_subtype_form. eauto. all: inv H8.
+  inv wfa'. inv H6. inv H7. eapply VeqHandler.
+  eapply ctx_subtype_form. eauto.
   - apply WfCtxU; auto.
   - apply SubtypeCtxU; auto. apply ctx_subtype_refl. auto.
   - eapply heq_subtype; eauto.
@@ -129,75 +136,82 @@ inv H1.
 + clear veq_subtype ceq_subtype. inv stya. apply ηUnit.
 + clear veq_subtype ceq_subtype. inv stya. apply ηFun.
 }{
-intros wfc' styc. inv orig. inv H.
-assert (wf_ctx Γ) as wfctx by (inv H5; assumption).
+intros same wfc' styc.
+assert (wf_ctx Γ) as wfctx.
+{ clear veq_subtype ceq_subtype. inv orig. inv H. inv H5. auto. } 
 assert (has_ctype Γ c1 C') as ty1.
-{ apply TypeC; auto. eapply TypeCSubtype; eauto. }
+{ clear veq_subtype ceq_subtype. inv orig. inv H.
+  apply TypeC; auto. eapply TypeCSubtype; eauto. }
 assert (has_ctype Γ c2 C') as ty2.
-{ apply TypeC; auto. eapply TypeCSubtype; eauto. }
+{ clear veq_subtype ceq_subtype. inv orig. inv H.
+  apply TypeC; auto. eapply TypeCSubtype; eauto. }
 apply WfForm; auto. apply WfCeq; auto.
-inv H1.
-+ specialize (ceq_subtype _ C' _ _ _ _ H4) as IH.
+{ clear veq_subtype ceq_subtype. inv orig. auto. }
+destruct orig. destruct H1; inv same.
++ specialize (ceq_subtype _ _ _ H1) as IH.
   clear veq_subtype ceq_subtype.
   apply CeqSym. eauto.
-+ specialize (ceq_subtype _ C' _ _ _ _ H6) as IH1.
-  specialize (ceq_subtype _ C' _ _ _ _ H9) as IH2.
++ specialize (ceq_subtype _ _ _ H1) as IH1.
+  specialize (ceq_subtype _ _ _ H2) as IH2.
   clear veq_subtype ceq_subtype.
   eapply CeqTrans; eauto.
 + inv styc.
-  specialize (veq_subtype _ A' _ _ _ _ H4) as IH.
+  specialize (veq_subtype _ _ _ H1) as IH.
   clear veq_subtype ceq_subtype.
   inv wfc'. eapply CeqRet; eauto.
 + clear veq_subtype ceq_subtype.
   eapply CeqAbsurd; eauto.
-+ specialize (ceq_subtype _ C' _ _ _ _ H9) as IH.
++ specialize (ceq_subtype _ _ _ H2) as IH.
   clear veq_subtype ceq_subtype.
   eapply CeqΠMatch; eauto.
-+ specialize (ceq_subtype _ C' _ _ _ _ H9) as IH1.
-  specialize (ceq_subtype _ C' _ _ _ _ H10) as IH2.
++ specialize (ceq_subtype _ _ _ H2) as IH1.
+  specialize (ceq_subtype _ _ _ H3) as IH2.
   clear veq_subtype ceq_subtype.
   eapply CeqΣMatch; eauto.
-+ specialize (ceq_subtype _ C' _ _ _ _ H9) as IH1.
-  specialize (ceq_subtype _ C' _ _ _ _ H10) as IH2.
++ specialize (ceq_subtype _ _ _ H2) as IH1.
+  specialize (ceq_subtype _ _ _ H3) as IH2.
   clear veq_subtype ceq_subtype.
   eapply CeqListMatch; eauto.
 + inv styc. rename A' into B'.
-  specialize (ceq_subtype _ (CTy A Σ' E') _ _ _ _ H6) as IH1.
-  specialize (ceq_subtype _ (CTy B' Σ' E') _ _ _ _ H9) as IH2.
+  specialize (ceq_subtype _ _ _ H1) as IH1.
+  specialize (ceq_subtype _ _ _ H2) as IH2.
   clear veq_subtype ceq_subtype.
-  assert (wf_vtype A) by (inv H6; inv H; inv H12; inv H4; inv H1; auto).
+  assert (wf_vtype A).
+  { inv H1. inv H3. inv H11. inv H3. auto. }
   eapply CeqDoBind.
-  - apply IH1. apply WfCTy; eauto; inv wfc'; auto.
+  - eapply IH1. eauto. apply WfCTy; eauto; inv wfc'; auto.
     apply SubtypeCTy; auto. apply vsubtype_refl. auto.
-  - apply IH2; eauto. apply SubtypeCTy; auto.
-+ specialize (veq_subtype _ (TyFun A C') _ _ _ _ H6) as IH.
+  - eapply IH2; eauto. apply SubtypeCTy; auto.
++ specialize (veq_subtype _ _ _ H1) as IH.
   clear veq_subtype ceq_subtype.
-  assert (wf_vtype A) by (inv H6; inv H; inv H8; inv H3; inv H1; auto).
-  eapply CeqApp; eauto. apply IH.
+  assert (wf_vtype A).
+  { inv H2. inv H3. inv H8. auto. }
+  eapply CeqApp; eauto. eapply IH. eauto.
   - apply WfTyFun; assumption.
   - apply SubtypeTyFun. apply vsubtype_refl. all: auto.
 + rename C' into D'.
-  specialize (veq_subtype _ (TyHandler C0 D') _ _ _ _ H6) as IH.
+  specialize (veq_subtype _ _ _ H1) as IH.
   clear veq_subtype ceq_subtype.
-  assert (wf_ctype C0) by (inv H6; inv H; inv H8; inv H3; inv H1; auto).
-  eapply CeqHandle; eauto. apply IH.
+  assert (wf_ctype C0).
+  { inv H1. inv H3. inv H8. inv H3. auto. }
+  eapply CeqHandle; eauto. eapply IH. eauto.
   - apply WfTyHandler; assumption.
   - apply SubtypeTyHandler. apply csubtype_refl. all: auto.
 + rename C' into D'.
-  specialize (ceq_subtype _ D' _ _ _ _ H9) as IH.
+  specialize (ceq_subtype _ _ _ H2) as IH.
   clear veq_subtype ceq_subtype.
   eapply CeqLetRec; eauto.
-+ inv styc.
-  eapply sig_subtype_get_Some in H6 as getop; eauto.
-  destruct getop as [A_op'[B_op'[gets[asty bsty]]]].
-  specialize (veq_subtype _ A_op' _ _ _ _ H9) as IH1.
-  specialize (ceq_subtype _ (CTy A' Σ' E') _ _ _ _ H10) as IH2.
++ specialize (veq_subtype _ _ _ H2) as IH1.
+  specialize (ceq_subtype _ _ _ H3) as IH2.
   clear veq_subtype ceq_subtype.
+  inv styc.
+  eapply sig_subtype_get_Some in H9 as getop; eauto.
+  destruct getop as [A_op'[B_op'[gets[asty bsty]]]].
   eapply CeqOp; eauto; inv wfc'.
-  - apply IH1.
+  - eapply IH1. eauto.
     eapply get_op_type_wf in gets. destruct gets. all: auto.
   - eapply ctx_subtype_form; eauto.
-    * apply IH2. apply WfCTy; eauto. apply SubtypeCTy; auto.
+    * eapply IH2. eauto. apply WfCTy; eauto. apply SubtypeCTy; auto.
     * apply WfCtxU. auto. 
       eapply get_op_type_wf in gets. destruct gets. all: auto.
     * eapply SubtypeCtxU. apply ctx_subtype_refl. all: auto.
@@ -229,13 +243,13 @@ inv H1.
   eapply βHandle_Op. eauto.
 + clear veq_subtype ceq_subtype.
   eapply ηPair. omega.
-  apply TypeC. inv H9. eauto. auto. eapply TypeCSubtype; eauto.
+  apply TypeC. inv H2. eauto. auto. eapply TypeCSubtype; eauto.
 + clear veq_subtype ceq_subtype.
   eapply ηSum. omega.
-  apply TypeC. inv H9. eauto. auto. eapply TypeCSubtype; eauto.
+  apply TypeC. inv H2. eauto. auto. eapply TypeCSubtype; eauto.
 + clear veq_subtype ceq_subtype.
   eapply ηList. omega.
-  apply TypeC. inv H9. eauto. auto. eapply TypeCSubtype; eauto.
+  apply TypeC. inv H2. eauto. auto. eapply TypeCSubtype; eauto.
 + clear veq_subtype ceq_subtype.
   eapply ηDoBind.
 }
@@ -243,12 +257,12 @@ Qed.
 
 (* ==================== Structural Rules for Cases ==================== *)
 
-Lemma heq_case_extend_trivial Σ D Γ h1 h2 op A1 A2 B1 B2 c1 c2:
-  heq Σ D Γ h1 h2 ->
+Lemma heq_case_extend_trivial Σ D Γ Ψ h1 h2 op A1 A2 B1 B2 c1 c2:
+  form Γ Ψ (Heq Σ D h1 h2) ->
   get_case h1 op = None -> get_case h2 op = None ->
   has_ctype (CtxU (CtxU Γ (TyFun B1 D)) A1) c1 D ->
   has_ctype (CtxU (CtxU Γ (TyFun B2 D)) A2) c2 D ->
-  heq Σ D Γ (CasesU h1 op c1) (CasesU h2 op c2).
+  form Γ Ψ (Heq Σ D (CasesU h1 op c1) (CasesU h2 op c2)).
 Proof.
 intros orig f1 f2 tys1 tys2.
 assert (wf_vtype A1) as wfa1 by (inv tys1; inv H; auto).
@@ -256,93 +270,99 @@ assert (wf_vtype A2) as wfa2 by (inv tys2; inv H; auto).
 assert (wf_vtype B1) as wfb1 by (inv tys1; inv H; inv H4; inv H6; auto).
 assert (wf_vtype B2) as wfb2 by (inv tys2; inv H; inv H4; inv H6; auto).
 assert (wf_ctype D) as wfd by (inv tys1; auto).
-assert (wf_ctx Γ) as wfctx by (inv orig; inv H2; auto).
-destruct orig.
+assert (wf_ctx Γ) as wfctx by (inv orig; inv H; inv H10; auto).
+inv orig. inv H.
 assert (get_op_type Σ1 op = None) as getn1.
 { destruct (get_op_type Σ1 op) eqn: g. destruct p. 2: reflexivity.
-  eapply h_has_case in H2; eauto. destruct H2 as [c f].
+  eapply h_has_case in H10; eauto. destruct H10 as [c f].
   rewrite f in f1. discriminate. }
 assert (get_op_type Σ2 op = None) as getn2.
 { destruct (get_op_type Σ2 op) eqn: g. destruct p. 2: reflexivity.
-  eapply h_has_case in H3; eauto. destruct H3 as [c f].
+  eapply h_has_case in H11; eauto. destruct H11 as [c f].
   rewrite f in f2. discriminate. }
 assert (sig_subtype Σ (SigU Σ1 op A1 B1)) as ss1.
-{ apply sig_subtype_extend. auto. apply WfSigU; auto. inv H2. assumption. }
+{ apply sig_subtype_extend. auto. apply WfSigU; auto. inv H10. assumption. }
 assert (sig_subtype Σ (SigU Σ2 op A2 B2)) as ss2.
-{ apply sig_subtype_extend. auto. apply WfSigU; auto. inv H3. assumption. }
+{ apply sig_subtype_extend. auto. apply WfSigU; auto. inv H11. assumption. }
 induction Σ as [ | Σ IH o A B].
-+ eapply Heq. auto. exact ss1. exact ss2.
-  - apply TypeH. 2:apply WfSigU. 2:inv H2. 7:apply TypeCasesU. all: auto.
-  - apply TypeH. 2:apply WfSigU. 2:inv H3. 7:apply TypeCasesU. all: auto.
++ eapply WfForm; auto. eapply WfHeq. auto. exact ss1. exact ss2.
+  - apply TypeH. 2:apply WfSigU. 2:inv H10. 7:apply TypeCasesU. all: auto.
+  - apply TypeH. 2:apply WfSigU. 2:inv H11. 7:apply TypeCasesU. all: auto.
   - apply HeqSigØ.
-+ eapply Heq. auto. exact ss1. exact ss2.
-  - apply TypeH. 2:apply WfSigU. 2:inv H2. 7:apply TypeCasesU. all: auto.
-  - apply TypeH. 2:apply WfSigU. 2:inv H3. 7:apply TypeCasesU. all: auto.
-  - inv H4. eapply HeqSigU.
-    * simpl. destruct (o==op). rewrite e, f1 in H9. discriminate. eauto.
-    * simpl. destruct (o==op). rewrite e, f2 in H14. discriminate. eauto.
++ eapply WfForm; auto. eapply WfHeq. auto. exact ss1. exact ss2.
+  - apply TypeH. 2:apply WfSigU. 2:inv H10. 7:apply TypeCasesU. all: auto.
+  - apply TypeH. 2:apply WfSigU. 2:inv H11. 7:apply TypeCasesU. all: auto.
+  - inv H1. eapply HeqSigU.
+    * simpl. destruct (o==op). rewrite e, f1 in H12. discriminate. eauto.
+    * simpl. destruct (o==op). rewrite e, f2 in H16. discriminate. eauto.
     * assumption.
-    * inv H. inv H0. inv H1. inv H16.
-      apply IH; auto; apply sig_subtype_extend; auto.
-      all: inv H2; inv H3; apply WfSigU; auto.
+    * inv H18. inv H6. inv H8. inv H9.
+      apply IH; auto. 
+      all: apply sig_subtype_extend; auto.
+      all: apply WfSigU; auto. inv H10. auto. inv H11. auto.
 Qed.
 
 
-Lemma heq_case_extend_structural Σ D Γ h1 h2 op A B c1 c2:
-  heq Σ D Γ h1 h2 ->
+Lemma heq_case_extend_structural Σ D Γ Ψ h1 h2 op A B c1 c2:
+  form Γ Ψ (Heq Σ D h1 h2) ->
   get_case h1 op = None -> get_case h2 op = None ->
-  ceq D (CtxU (CtxU Γ (TyFun B D)) A) c1 c2 ->
-  heq (SigU Σ op A B) D Γ (CasesU h1 op c1) (CasesU h2 op c2).
+  form (CtxU (CtxU Γ (TyFun B D)) A) (hyp_shift Ψ 2 0) (Ceq D c1 c2) ->
+  form Γ Ψ (Heq (SigU Σ op A B) D (CasesU h1 op c1) (CasesU h2 op c2)).
 Proof.
 intros orig f1 f2 ceq12.
-assert (has_ctype (CtxU (CtxU Γ (TyFun B D)) A) c1 D) as tys1 
-by (inv ceq12; auto).
-assert (has_ctype (CtxU (CtxU Γ (TyFun B D)) A) c2 D) as tys2 
-by (inv ceq12; auto).
+assert (has_ctype (CtxU (CtxU Γ (TyFun B D)) A) c1 D) as tys1.
+{ inv ceq12. inv H. auto. }
+assert (has_ctype (CtxU (CtxU Γ (TyFun B D)) A) c2 D) as tys2.
+{ inv ceq12. inv H. auto. }
 assert (wf_vtype A) as wfa by (inv tys1; inv H; auto).
 assert (wf_vtype B) as wfb by (inv tys1; inv H; inv H4; inv H6; auto).
 assert (wf_ctype D) as wfd by (inv tys1; auto).
-assert (wf_ctx Γ) as wfctx by (inv orig; inv H2; auto).
-destruct orig.
+assert (wf_ctx Γ) as wfctx by (inv orig; inv H; inv H10; auto).
+inv orig. inv H.
 assert (get_op_type Σ1 op = None) as getn1.
 { destruct (get_op_type Σ1 op) eqn: g. destruct p. 2: reflexivity.
-  eapply h_has_case in H2; eauto. destruct H2 as [c f].
+  eapply h_has_case in H10; eauto. destruct H10 as [c f].
   rewrite f in f1. discriminate. }
 assert (get_op_type Σ2 op = None) as getn2.
 { destruct (get_op_type Σ2 op) eqn: g. destruct p. 2: reflexivity.
-  eapply h_has_case in H3; eauto. destruct H3 as [c f].
+  eapply h_has_case in H11; eauto. destruct H11 as [c f].
   rewrite f in f2. discriminate. }
 assert (sig_subtype (SigU Σ op A B) (SigU Σ1 op A B)) as ss1.
 { eapply SubtypeSigU. apply sig_subtype_extend. auto. apply WfSigU; auto. 
-  inv H2. auto. simpl. destruct (op==op). reflexivity. destruct n. auto.
+  inv H10. auto. simpl. destruct (op==op). reflexivity. destruct n. auto.
   all: apply vsubtype_refl; auto. }
 assert (sig_subtype (SigU Σ op A B) (SigU Σ2 op A B)) as ss2.
 { eapply SubtypeSigU. apply sig_subtype_extend. auto. apply WfSigU; auto. 
-  inv H3. auto. simpl. destruct (op==op). reflexivity. destruct n. auto.
+  inv H11. auto. simpl. destruct (op==op). reflexivity. destruct n. auto.
   all: apply vsubtype_refl; auto. }
 assert (get_op_type Σ op = None) as sgetnone.
 { destruct (get_op_type Σ op) eqn: gs; auto. destruct p.
-  eapply sig_subtype_get_Some in H0; eauto. destruct H0 as [a[b[g]]]. 
+  eapply sig_subtype_get_Some in H8; eauto. destruct H8 as [a[b[g]]]. 
   rewrite g in getn1. discriminate. }
-eapply Heq. apply WfSigU; auto. exact ss1. exact ss2.
-- apply TypeH. 2:apply WfSigU. 2:inv H2. 7:apply TypeCasesU. all: auto.
-- apply TypeH. 2:apply WfSigU. 2:inv H3. 7:apply TypeCasesU. all: auto.
+eapply WfForm; auto. eapply WfHeq. apply WfSigU; auto. exact ss1. exact ss2.
+- apply TypeH. 2:apply WfSigU. 2:inv H10. 7:apply TypeCasesU. all: auto.
+- apply TypeH. 2:apply WfSigU. 2:inv H11. 7:apply TypeCasesU. all: auto.
 - eapply HeqSigU.
   * simpl. destruct (op==op). reflexivity. destruct n. auto.
   * simpl. destruct (op==op). reflexivity. destruct n. auto.
   * assumption.
-  * eapply heq_case_extend_trivial; eauto. eapply Heq. 2:exact H0. all: eauto.
+  * eapply heq_case_extend_trivial; eauto. 
+    eapply WfForm. eapply WfHeq. 2:exact H8. all: eauto.
 Qed.
 
 (* ================== Reflexivity, Symmetry, Transitivity ================== *)
 
-Lemma veq_refl Γ v A   : has_vtype Γ v A -> veq A Γ v v
-with  ceq_refl Γ c C   : has_ctype Γ c C -> ceq C Γ c c
-with  heq_refl Γ h Σ D : has_htype Γ h Σ D -> heq Σ D Γ h h.
+Lemma veq_refl Γ v A : 
+  has_vtype Γ v A -> form Γ HypØ (Veq A v v)
+with ceq_refl Γ c C : 
+  has_ctype Γ c C -> form Γ HypØ (Ceq C c c)
+with heq_refl Γ h Σ D : 
+  has_htype Γ h Σ D -> form Γ HypØ (Heq Σ D h h).
 Proof.
 all: intros orig.
 {
-apply Veq; auto. all: destruct orig; auto. destruct H1.
+apply WfForm. apply WfVeq; auto. apply WfHypØ. inv orig. auto.
+destruct orig. destruct H1.
 + apply VeqUnit.
 + apply VeqInt. 
 + eapply VeqVar. eauto. apply vsubtype_refl. assumption.
@@ -351,11 +371,12 @@ apply Veq; auto. all: destruct orig; auto. destruct H1.
 + apply VeqInr; eauto.
 + apply VeqListNil; eauto.
 + apply VeqListCons; eauto.
-+ apply VeqFun; eauto.
++ apply VeqFun; eauto. 
 + eapply VeqHandler; eauto. apply csubtype_refl. inv H2. assumption.
 + apply veq_refl in H1. eapply veq_subtype in H1; eauto. inv H1. assumption.
 }{
-apply Ceq; auto. all: destruct orig; auto. destruct H1.
+apply WfForm. apply WfCeq; auto. apply WfHypØ. inv orig. auto.
+destruct orig. destruct H1.
 + apply CeqRet. auto.
 + apply CeqAbsurd. auto.
 + eapply CeqΠMatch; eauto.
@@ -368,10 +389,11 @@ apply Ceq; auto. all: destruct orig; auto. destruct H1.
 + eapply CeqOp; eauto.
 + apply ceq_refl in H1. eapply ceq_subtype in H1; eauto. inv H1. assumption.
 }{
-eapply Heq. inv orig. assumption.
+apply WfForm. eapply WfHeq; auto.
+inv orig. assumption.
 apply sig_subtype_refl. inv orig. assumption.
 apply sig_subtype_refl. inv orig. assumption.
-assumption. assumption.
+assumption. assumption. apply WfHypØ. inv orig. assumption.
 destruct orig. destruct H2.
 + eapply HeqSigØ.
 + assert (get_case (CasesU h op cop) op = Some cop).
@@ -382,47 +404,69 @@ destruct orig. destruct H2.
 Qed.
 
 
-Lemma veq_sym A Γ v1 v2   : veq A Γ v1 v2 -> veq A Γ v2 v1
-with  ceq_sym C Γ c1 c2   : ceq C Γ c1 c2 -> ceq C Γ c2 c1
-with  heq_sym Σ D Γ h1 h2 : heq Σ D Γ h1 h2 -> heq Σ D Γ h1 h2.
+Lemma veq_sym A Γ Ψ v1 v2 : 
+  form Γ Ψ (Veq A v1 v2) -> form Γ Ψ (Veq A v2 v1)
+with ceq_sym C Γ Ψ c1 c2 : 
+  form Γ Ψ (Ceq C c1 c2) -> form Γ Ψ (Ceq C c2 c1).
 Proof.
 {
-intro orig. apply Veq. all: try (inv orig; assumption). apply VeqSym. auto.
+intro orig. apply WfForm. apply WfVeq. all: try (inv orig; inv H; assumption).
+apply VeqSym. auto.
 }{
-intro orig. apply Ceq. all: try (inv orig; assumption). apply CeqSym. auto.
+intro orig. apply WfForm. apply WfCeq. all: try (inv orig; inv H; assumption).
+apply CeqSym. auto.
+}
+Qed.
+
+Lemma heq_sym Σ D Γ Ψ h1 h2 : 
+  form Γ Ψ (Heq Σ D h1 h2) -> form Γ Ψ (Heq Σ D h2 h1).
+Proof.
+induction Σ; intros orig.
+all: apply WfForm; try (inv orig; assumption).
++ inv orig. inv H. eapply WfHeq. auto.
+  exact H9. exact H8. all: eauto.
++ apply HeqSigØ.
++ inv orig. inv H. eapply WfHeq. auto.
+  exact H9. exact H8. all: eauto. 
++ inv orig. inv H1. eapply HeqSigU; eauto.
+  apply ceq_sym. auto.
+Qed.
+
+    
+Lemma veq_trans A Γ Ψ v1 v2 v3:
+  form Γ Ψ (Veq A v1 v2) -> form Γ Ψ (Veq A v2 v3) -> form Γ Ψ (Veq A v1 v3)
+
+with  ceq_trans C Γ Ψ c1 c2 c3:
+  form Γ Ψ (Ceq C c1 c2) -> form Γ Ψ (Ceq C c2 c3) -> form Γ Ψ (Ceq C c1 c3).
+
+Proof.
+{
+intros veq1 veq2. apply WfForm. apply WfVeq. 
++ inv veq1. inv H. auto.
++ inv veq2. inv H. auto.
++ inv veq1. auto.
++ eapply VeqTrans; eauto.
 }{
-intro orig. destruct orig. induction H4.
-+ eapply Heq. 2: exact H0. all: eauto. apply HeqSigØ.
-+ eapply Heq. 2: exact H0. all: eauto.
-  eapply HeqSigU; eauto.
+intros ceq1 ceq2. apply WfForm. apply WfCeq. 
++ inv ceq1. inv H. auto.
++ inv ceq2. inv H. auto.
++ inv ceq1. auto.
++ eapply CeqTrans; eauto.
 }
 Qed.
 
 
-Lemma veq_trans A Γ v1 v2 v3:
-  veq A Γ v1 v2 -> veq A Γ v2 v3 -> veq A Γ v1 v3
-
-with  ceq_trans C Γ c1 c2 c3:
-  ceq C Γ c1 c2 -> ceq C Γ c2 c3 -> ceq C Γ c1 c3
-
-with  heq_trans Σ D Γ h1 h2 h3:
-  heq Σ D Γ h1 h2 -> heq Σ D Γ h2 h3 -> heq Σ D Γ h1 h3.
-
-Proof.
+Lemma heq_trans Σ D Γ Ψ h1 h2 h3:
+  form Γ Ψ (Heq Σ D h1 h2) -> form Γ Ψ (Heq Σ D h2 h3) -> 
+  form Γ Ψ (Heq Σ D h1 h3).
 {
-intros veq1 veq2. apply Veq. inv veq1. auto. inv veq2. auto.
-eapply VeqTrans; eauto.
-}{
-intros ceq1 ceq2. apply Ceq. inv ceq1. auto. inv ceq2. auto.
-eapply CeqTrans; eauto.
-}{
-intros heq1 heq2. induction Σ. 
-+ inv heq1. inv heq2. eapply Heq. 2: exact H0. all: eauto. apply HeqSigØ.
-+ inv heq1. inv heq2. eapply Heq. 2: exact H0. all: eauto.
-  inv H4. inv H10. eapply HeqSigU; eauto.
-  rewrite H14 in H20. inv H20. apply Ceq.
-  - inv H21. assumption.
-  - inv H24. assumption.
-  - eapply CeqTrans; eauto.
+intros heq1 heq2. induction Σ.
++ inv heq1. inv heq2. inv H. inv H2. eapply WfForm. eapply WfHeq.
+  2: exact H11. 2: exact H16. all: eauto. apply HeqSigØ.
++ inv heq1. inv heq2. inv H. inv H2. eapply WfForm. eapply WfHeq.
+  2: exact H11. 2: exact H16. all: eauto. 
+  inv H1. inv H4. eapply HeqSigU; eauto.
+  rewrite H10 in H23. inv H23.
+  eapply ceq_trans; eauto.
 }
 Qed.
