type_system/subtyping.v
@@ -49,3 +49,10 @@ Inductive ctx_subtype : ctx -> ctx -> Prop :=
     ctx_subtype Γ Γ' -> vsubtype A A' -> 
     ctx_subtype (CtxU Γ A) (CtxU Γ' A')
 .
+
+Inductive hyp_subset : hypotheses -> hypotheses -> Prop :=
+| SubsetHypØ Ψ : hyp_subset HypØ Ψ
+| SubsetHypU Ψ φ Ψ' : 
+    hyp_subset Ψ Ψ' ->
+    has_hypothesis Ψ φ ->
+    hyp_subset (HypU Ψ φ) Ψ'. 
